cfrontend/SemanticsProofs.v
@@ -1,35 +1,99 @@
 Require Import Coqlib Errors Maps.
-Require Import Integers Floats Values AST Memory Allocator Builtins Events Globalenvs Tags.
+Require Import Integers Floats Values AST Memory Allocator.
+Require Import Builtins Events Globalenvs Tags.
 Require Import Ctypes Cop Csyntax Csem.
-Require Import Smallstep.
+Require Import Smallstep Simulation.
 Require Import List. Import ListNotations.
 Require Import String.
+Require Import Coq.Logic.Eqdep_dec.
+Require Import NullPolicy.
 
-Module PolicyInsensitivity (Ptr: Pointer) (Pol1: Policy) (Pol2: Policy)
+Module PolicyInsensitivity (Ptr: Pointer) (Pol: Policy)
        (M: Memory Ptr) (A: Allocator Ptr).
-  Module M1 := M Pol1.
-  Module M2 := M Pol2.
-  Module A1 := A Pol1 M1.
-  Module A2 := A Pol2 M2.
-  Module Csem1 := Csem Ptr Pol1 M1 A1.
-  Module Csem2 := Csem Ptr Pol2 M2 A2.
-
-  Module PE := ProgEquiv Ptr Pol1 M1 A1
-                         Ptr Pol2 M2 A2.
+  Module M1 := M Pol.
+  Module M2 := M NullPolicy.
+  Module A1 := A Pol M1.
+  Module A2 := A NullPolicy M2.
+  Module FS := FSIM Ptr Pol M1 A1
+                    Ptr NullPolicy M2 A2.
+  Import FS.
   Import PE.
   
   Variable prog1 : CS1.program.
   Variable prog2 : CS2.program.
-  
-  Axiom same_prog : prog_match prog1 prog2.
 
-  Print Csem1.semantics.
+  Definition gcm1 := Csem1.globalenv prog1.
+  Definition gcm2 := Csem2.globalenv prog2.
+
+  Variable ce : composite_env.
+  Variable ge1 : Csem1.Smallstep.Events.Genv.t
+                   Csem1.Csyntax.fundef type.
+  Variable m1 : CS1.Cop.Events.Genv.mem.
+  Variable ge2 : Csem2.Smallstep.Events.Genv.t
+                   Csem2.Csyntax.fundef type.
+  Variable m2 : CS2.Cop.Events.Genv.mem.
+  Variable sem1 : S1.semantics.
+  Variable sem2 : S2.semantics.
+
+  Hypothesis same_prog : prog_match prog1 prog2.
+
+  Hypothesis globalenv1 :
+    Csem1.globalenv prog1 = MemorySuccess (ge1,ce,m1).
   
-  Theorem PolicyInsensitive :
+  Hypothesis sem1_src : Csem1.semantics prog1 ge1 ce = sem1.
+  Hypothesis sem2_src : Csem2.semantics prog2 ge2 ce = sem2.
+  
+  (* Define matching relation on states that holds if they match except for tags.*)
+  Print Csem1.state.
+  Inductive match_states : Csem1.state -> Csem2.state -> Prop :=
+  | MState : forall f1 f2 pct1 pct2 stmt1 stmt2 k1 k2 e1 e2 te1 te2 m1 m2,
+      match_states (Csem1.State f1 pct1 stmt1 k1 e1 te1 m1)
+                   (Csem2.State f2 pct2 stmt2 k2 e2 te2 m2)
+  | MExprState : forall f1 f2 l pct1 pct2 expr1 expr2 k1 k2 e1 e2 te1 te2 m1 m2,
+      match_states (Csem1.ExprState f1 l pct1 expr1 k1 e1 te1 m1)
+                   (Csem2.ExprState f2 l pct2 expr2 k2 e2 te2 m2)      
+  | MCallstate : forall fd1 fd2 l pct1 pct2 fpt1 fpt2 args1 args2 k1 k2 m1 m2,
+      match_states (Csem1.Callstate fd1 l pct1 fpt1 args1 k1 m1)
+                   (Csem2.Callstate fd2 l pct2 fpt2 args2 k2 m2)
+  | MReturnState : forall fd1 fd2 l pct1 pct2 retv1 retv2 k1 k2 m1 m2,
+      match_states (Csem1.Returnstate fd1 l pct1 retv1 k1 m1)
+                   (Csem2.Returnstate fd2 l pct2 retv2 k2 m2)  
+  | MStuckstate : match_states Csem1.Stuckstate Csem2.Stuckstate
+  | Failstop : forall s2 msg failure,
+      match_states (Csem1.Failstop msg failure [])
+                   s2
+  .
+  
+  Theorem PolicyInsensitiveForward : forward_simulation sem1 sem2.
+  Proof.
+    pose proof sem1_src.
+    unfold Csem1.semantics in *.
+    rewrite <- H. clear H.
+    pose proof sem2_src.
+    unfold Csem2.semantics in *.
+    rewrite <- H. clear H.
+
+    (*pose proof same_prog. inv H. pose proof success1. pose proof success2.*)
+    (* prog_defs1&2 contain matching, but not equal, function bodies *)
+    eapply forward_simulation_step; simpl.
+    - admit. (* Need to show that, if prog_defs match, the same symbols are found
+                in gv find_symb. *)
+    - admit. (* Need to show that state is equivalent to Csem1.state and state0
+                is Csem2.state. Destruct on (initial_state s1) and construct an
+                s2 such that (initial_state s2) but with other tags, so matching.*)
+    - admit. (* Need to show that state is equivalent to Csem1.state and state0
+                is Csem2.state. Destruct on (initial_state s1) and construct an
+                s2 such that (final_state s2) but with other tags, so matching.*)
+    - instantiate (1 := match_states). intros. inv H0.
+      inv H. inv H0. inv H0. eexists. eexists. intuition.
+      econstructor.
+      admit. (* Need to show that state is equivalent to Csem1.state and state0
+                is Csem2.state. Destruct and apply rules. *)
+    Admitted.
   
 End PolicyInsensitivity.
 
-  Module Compartmentalization (Ptr: Pointer) (Pol: Policy)
+Module Compartmentalization (Ptr: Pointer) (Pol: Policy)
        (M: Memory) (A: Allocator).
   Module Ctop := Ctop Ptr.
   Module Csem := Csem Ptr Pol M A.
